QuantumLean/Hadamard.lean
@@ -20,13 +20,13 @@ def H : nMatrix 1 := !![1, 1; 1, -1]
 def Hadamard (n : ℕ) := pow_kronecker n H
 
 
-theorem hadamard_Identity : H * H = (2 : ℕ) := by
+theorem H_mul_H_1 : H * H = (2 : ℕ) := by
   simp [H, mul_apply, ofNat_fin_two]
   norm_num
 
 
 theorem H_mul_H : Hadamard n * Hadamard n = (2 ^ n : ℕ) := by
-  rw [Hadamard, ← pow_kronecker_mul, hadamard_Identity, pow_kronecker_of_natCast]
+  rw [Hadamard, ← pow_kronecker_mul, H_mul_H_1, pow_kronecker_of_natCast]
 
 end Hadamard
 
